Add comments

Nonlinear_Arithmetic/Power2.dfy
@@ -11,111 +11,116 @@ module Power2 {
   import opened MulInternals
   import opened Power
 
-  function method {:opaque} power2(exp: nat): nat
-    ensures power2(exp) > 0
+  function method {:opaque} power2(e: nat): nat
+    ensures power2(e) > 0
   {
-    if exp == 0 then
+    if e == 0 then
       1
     else
-      2 * power2(exp-1)
+      2 * power2(e-1)
   }
 
+  /* power2() is equivalent to power() with a base of 2. */
   lemma lemma_power2_is_power_2_auto()
-    ensures forall x: nat :: power2(x) == power(2, x)
+    ensures forall e: nat {:trigger power2(e)} :: power2(e) == power(2, e)
   {
     reveal power2();
     reveal power();
     
-    forall x: nat
-      ensures power2(x) == power(2,x)
+    forall e: nat {:trigger power2(e)}
+      ensures power2(e) == power(2, e)
     {
-      lemma_power2_is_power_2(x);
+      lemma_power2_is_power_2(e);
     }
   }
 
-  lemma lemma_power2_is_power_2(x: nat)
-    ensures power2(x) == power(2, x)
+  /* power2() is equivalent to power() with base 2. */
+  lemma lemma_power2_is_power_2(e: nat)
+    ensures power2(e) == Power.power(2, e)
   {
-    reveal power();
+    reveal Power.power();
     reveal power2();
-    if x != 0 {
-      lemma_power2_is_power_2(x-1);
+    if e != 0 {
+      lemma_power2_is_power_2(e-1);
     }
   }
 
-  lemma lemma_power2_auto()
+  /* Properties of powers with base 2. */
+  lemma lemma_auto()
     ensures power2(0) == 1
     ensures power2(1) == 2
-    ensures forall x: nat, y: nat {:trigger power2(x+y)} :: power2(x+y) == power2(x) * power2(y)
-    ensures forall x: nat, y: nat {:trigger power2(x-y)} :: x >= y ==> power2(x-y) * power2(y) == power2(x)
-    // ensures forall x: nat, y: nat {:trigger x*y} :: y == 2 ==> x*y == x+x
+    ensures forall e1: nat, e2: nat {:trigger power2(e1+e2)} :: power2(e1+e2) == power2(e1) * power2(e2)
+    ensures forall e1: nat, e2: nat {:trigger power2(e1-e2)} :: e1 >= e2 ==> power2(e1-e2) * power2(e2) == power2(e1)
   {
     reveal power2();
     lemma_power2_is_power_2_auto();
-    lemma_power_auto();
+    Power.lemma_auto();
   }
 
-  //////////////////////////////////////////////////////////////////////////////
-
-  lemma lemma_power2_strictly_increases(e1: int, e2: int)
+  /* 2 raised to a power strictly increases as the power strictly increases. */
+  lemma lemma_strictly_increases(e1: int, e2: int)
     requires 0 <= e1 < e2
     ensures power2(e1) < power2(e2)
   {
-    lemma_power2_auto();
+    lemma_auto();
     lemma_mul_induction_auto(e2-e1, e => 0 < e ==> power2(e1) < power2(e1+e));
   }
 
-  lemma lemma_power2_increases(e1: int, e2: int)
+  /* 2 raised to a power increases as the power increases. */
+  lemma lemma_increases(e1: int, e2: int)
     requires 0 <= e1 <= e2
     ensures power2(e1) <= power2(e2)
   {
-    lemma_power2_auto();
-    lemma_mul_induction_auto(e2 - e1, e => 0 <= e ==> power2(e1) <= power2(e1 + e));
+    lemma_auto();
+    lemma_mul_induction_auto(e2-e1, e => 0 <= e ==> power2(e1) <= power2(e1+e));
   }
 
-  lemma lemma_power2_strictly_increases_converse(e1: int, e2: int)
+  /* A power strictly increases as 2 raised to the power strictly increases. */
+  lemma lemma_strictly_increases_converse(e1: int, e2: int)
     requires 0 <= e1
     requires 0 < e2
     requires power2(e1) < power2(e2)
     ensures e1 < e2
   {
-    if (e1 >= e2)
-    {
-      lemma_power2_increases(e2, e1);
+    if e1 >= e2 {
+      lemma_increases(e2, e1);
       assert false;
     }
   }
 
-  lemma lemma_power2_increases_converse(e1: int, e2: int)
+  /* A power increases as 2 raised to the power increases. */
+  lemma lemma_increases_converse(e1: int, e2: int)
     requires 0 < e1
     requires 0 < e2
     requires power2(e1) <= power2(e2)
     ensures e1 <= e2
   {
-    if (e1 > e2) {
-      lemma_power2_strictly_increases(e2, e1);
+    if e1 > e2 {
+      lemma_strictly_increases(e2, e1);
       assert false;
     }
   }
 
-  lemma lemma_power2_adds(e1:nat, e2:nat)
+  /* Add exponents when multiplying powers with base 2. */
+  lemma lemma_add(e1: nat, e2: nat)
     decreases e2
     ensures power2(e1 + e2) == power2(e1) * power2(e2)
   {
     reveal power2();
-    lemma_power2_auto();
+    lemma_auto();
   }
 
-  lemma lemma_power2_div_is_sub(x:int, y:int)
-    requires 0 <= x <= y
-    ensures power2(y - x) == power2(y) / power2(x) >= 0
+  /* Subtract exponents when dividing powers with base 2. */
+  lemma lemma_subtract(e1: int, e2: int)
+    requires 0 <= e1 <= e2
+    ensures power2(e2 - e1) == power2(e2)/power2(e1) >= 0
   {
     calc {
-      power2(y) / power2(x);
-        { lemma_power2_adds(y-x, x); }
-      (power2(y-x)*power2(x)) / power2(x);
-        { lemma_div_by_multiple(power2(y-x), power2(x)); }
-      power2(y-x);
+      power2(e2)/power2(e1);
+        { lemma_add(e2-e1, e1); }
+      power2(e2-e1)*power2(e1)/power2(e1);
+        { lemma_div_by_multiple(power2(e2-e1), power2(e1)); }
+      power2(e2-e1);
     }
   }
 
@@ -158,144 +163,119 @@ module Power2 {
     reveal power2();
   }
 
-  lemma lemma_power2_add8(n:int)
-    requires n >= 0
-    ensures power2(n + 1) == 2 * power2(n)
-    ensures power2(n + 2) == 4 * power2(n)
-    ensures power2(n + 3) == 8 * power2(n)
-    ensures power2(n + 4) == 16 * power2(n)
-    ensures power2(n + 5) == 32 * power2(n)
-    ensures power2(n + 6) == 64 * power2(n)
-    ensures power2(n + 7) == 128 * power2(n)
-    ensures power2(n + 8) == 256 * power2(n)
-  {
-    reveal power2();
-  }
-
+  /* 2^0 equals 1. */
   lemma lemma_power2_0_is_1()
     ensures power2(0) == 1
   {
     reveal power2();
   }
 
+  /* 2^1 equals 2. */
   lemma lemma_power2_1_is_2()
     ensures power2(1) == 2
   {
     reveal power2();
   }
 
-  lemma lemma_bit_count_is_unique(x:int, a:int, b:int)
-    requires 0<a
-    requires 0<b
+  /* If a number is in the ranges [2^(a-1), 2^a) and [2^(b-1), 2^b), then a is
+  equal to b. */
+  lemma lemma_bit_count_is_unique(x: int, a: int, b: int)
+    requires 0 < a
+    requires 0 < b
     requires power2(a-1) <= x < power2(a)
     requires power2(b-1) <= x < power2(b)
-    ensures a==b
+    ensures a == b
   {
-    if (a<b)
-    {
-      lemma_power2_increases(a,b-1);
+    if a < b {
+      lemma_increases(a, b-1);
       assert false;
     }
-    if (b<a)
-    {
-      lemma_power2_increases(b,a-1);
+    if b < a {
+      lemma_increases(b, a-1);
       assert false;
     }
   }
 
-  lemma lemma_pull_out_powers_of_2(x:nat, y:nat, z:nat)
-    ensures 0<=x*y
-    ensures 0<=y*z
+  /* (2^xy)^z = (2^x)^yz */
+  lemma lemma_pull_out_powers_of_2(x: nat, y: nat, z: nat)
+    ensures 0 <= x*y
+    ensures 0 <= y*z
     ensures power(power2(x*y), z) == power(power2(x), y*z)
   {
-    lemma_mul_nonnegative(x,y);
-    lemma_mul_nonnegative(y,z);
-    lemma_power_positive(2,x);
+    lemma_mul_nonnegative(x, y);
+    lemma_mul_nonnegative(y, z);
+    Power.lemma_positive_base(2, x);
     calc {
       power(power2(x*y), z);
         { lemma_power2_is_power_2(x*y); }
-      power(power(2,x*y), z);
-        { lemma_power_multiplies(2, x, y); }
-      power(power(power(2,x),y), z);
-        { lemma_power_multiplies(power(2,x), y, z); }
-      power(power(2,x), y*z);
+      power(power(2, x*y), z);
+        { Power.lemma_multiply(2, x, y); }
+      power(power(power(2, x), y), z);
+        { Power.lemma_multiply(power(2, x), y, z); }
+      power(power(2, x), y*z);
         { lemma_power2_is_power_2(x); }
       power(power2(x), y*z);
     }
   }
 
-  lemma lemma_rebase_powers_of_2()
-    ensures forall n:nat, e:nat {:trigger power(power2(n), e)} :: 0 <= n * e && power(power2(n), e) == power2(n * e)
+  /* Multiply exponents to find the power of a power of 2. */
+  lemma lemma_multiply_auto()
+    ensures forall n: nat, e: nat {:trigger power(power2(n), e)} :: 0 <= n * e && power(power2(n), e) == power2(n * e)
   {
     reveal power();
     reveal power2();
 
-    forall n:nat, e:nat
+    forall n: nat, e: nat
       ensures 0 <= n * e && power(power2(n), e) == power2(n * e)
     {
       lemma_pull_out_powers_of_2(1, n, e);
-      lemma_power2_auto();
+      lemma_auto();
       lemma_power2_is_power_2_auto();
     }
   }
 
-  lemma lemma_mask_div_2(c:nat)
-    requires 0<c
-    ensures (power2(c)-1)/2 == power2(c-1)-1
+  /* (2^e - 1)/2 = 2^(e-1) - 1 */
+  lemma lemma_mask_div_2(e: nat)
+    requires 0 < e
+    ensures (power2(e)-1)/2 == power2(e-1)-1
   {
-    lemma_power2_auto();
-    var f := u => 0 < u ==> (power2(u)-1)/2 == power2(u-1)-1;
+    lemma_auto();
+    var f := e => 0 < e ==> (power2(e)-1)/2 == power2(e-1)-1;
     assert forall i {:trigger is_le(0, i)} :: is_le(0, i) && f(i) ==> f(i + 1);
     assert forall i {:trigger is_le(i, 0)} :: is_le(i, 0) && f(i) ==> f(i - 1);
-    lemma_mul_induction_auto(c, f);
+    lemma_mul_induction_auto(e, f);
   }
 
-  lemma lemma_power2_division_inequality(x:nat, p:nat, s:nat)
-    requires s<=p
-    requires x<power2(p)
-    ensures x/power2(s) < power2(p-s)
+  /* Inequality due to smaller numerator, same denominator. */
+  lemma lemma_division_inequality(x: nat, e1: nat, e2: nat)
+    requires e2 <= e1
+    requires x < power2(e1)
+    ensures x/power2(e2) < power2(e1-e2)
   {
     calc ==> {
-      x/power2(s) >= power2(p-s);
-        { lemma_mul_inequality(power2(p-s), x/power2(s), power2(s)); }
-      (x/power2(s))*power2(s) >= power2(p-s)*power2(s);
-        { lemma_fundamental_div_mod(x, power2(s));
+      x/power2(e2) >= power2(e1-e2);
+        { lemma_mul_inequality(power2(e1-e2), x/power2(e2), power2(e2)); }
+      x/power2(e2)*power2(e2) >= power2(e1-e2)*power2(e2);
+        { lemma_fundamental_div_mod(x, power2(e2));
           lemma_mul_is_commutative_auto(); }
-      x - x%power2(s) >= power2(p-s)*power2(s);
-        { lemma_power2_adds(p-s, s); }
-      x - x%power2(s) >= power2(p);
+      x - x%power2(e2) >= power2(e1-e2)*power2(e2);
+        { lemma_add(e1-e2, e2); }
+      x - x%power2(e2) >= power2(e1);
         { lemma_mod_properties(); }
-      x >= power2(p);
+      x >= power2(e1);
       false;
     }
   }
 
-  lemma lemma_power2_unfolding(a:nat, b:nat)
-    ensures 0<=a*b
-    ensures power(power2(a), b) == power2(a*b)
+  /* Multiply exponents to find the power of a power of 2. */
+  lemma lemma_multiply(e1: nat, e2: nat)
+    ensures 0 <= e1*e2
+    ensures power(power2(e1), e2) == power2(e1*e2)
   {
-    lemma_mul_nonnegative(a,b);
-    lemma_power2_is_power_2(a);
-    lemma_power_multiplies(2,a,b);
-    lemma_power2_is_power_2(a*b);
-  }
-
-  function{:opaque} NatNumBits(n:nat):nat
-    ensures NatNumBits(n) >= 0
-  {
-    if n == 0 then 0 else 1 + NatNumBits(n / 2)
-  }
-
-  lemma lemma_Power2BoundIsNatNumBits(c:nat, n:nat)    
-    ensures (((c>0) ==> (power2(c-1) <= n)) && (n < power2(c))) <==> c == NatNumBits(n)
-  {
-    reveal NatNumBits();
-    reveal power2();
-    if (c > 0)
-    {
-      lemma_Power2BoundIsNatNumBits(c - 1, n / 2);
-    }
-    assert NatNumBits(n / 2) >= 0; //- dafnycc
+    lemma_mul_nonnegative(e1, e2);
+    lemma_power2_is_power_2(e1);
+    Power.lemma_multiply(2, e1, e2);
+    lemma_power2_is_power_2(e1*e2);
   }
 
 } 
